implement a mm checker

theories/mm.v
@@ -1,7 +1,7 @@
-From Coq Require Import String List.
+From Coq Require Import String List Arith Bool.
 Import ListNotations.
 
-Module Model.
+Section Model.
 
 Inductive Symbol :=
   | Var (v : nat)
@@ -39,5 +39,188 @@ Inductive Deduce (Ω : Universe) : Context -> Term -> Prop :=
 
 Notation "U , G ⊢ t" := (Deduce U G t) (at level 80).
 
+Definition Ω := [PROP [] [Cst "a"; Var 0]].
+Definition τ := [Cst "a"; Cst "b"].
+
+Goal Ω, [] ⊢ τ.
+Proof.
+  eapply (rule_instance _ _ _ (fun _ => [Cst "b"])).
+  + now constructor.
+  + reflexivity.
+  + now intros.
+Qed.
+
 End Model.
 
+
+Section Mm.
+
+Inductive Label :=
+  | TypeLbl (lbl : nat)
+  | FactLbl (lbl : nat)
+  | RuleLbl (lbl : nat).
+
+Inductive Statement :=
+  | Ax (stmt : Term)
+  | Th (stmt : Term) (proof : list Label).
+
+Record Rule := RULE {
+  type_hypothesis : list (nat * (string * nat));
+  fact_hypothesis : list (nat * Term);
+  statement    : Statement;
+}.
+
+Record File := FILE {
+  (* variables : list nat;
+  constants : list string; *)
+  rules     : list (nat * Rule);
+}.
+
+Fixpoint get {A} (l : list (nat * A)) (x : nat) : option A :=
+  match l with
+  | [] => None
+  | (y, vy)::xs =>
+    if (x =? y)%nat then
+      Some vy
+    else
+      get xs x
+  end.
+
+Definition Stack := list Term.
+Definition Binding : Type := (nat * Term).
+Definition Unifier := list Binding.
+
+Fixpoint binds (u : Unifier) (x : nat) :=
+  match u with
+  | [] => false
+  | (v, _)::u =>
+    (x =? v)%nat || binds u x
+  end.
+
+Fixpoint unify (Σ : Stack) (unifier : Unifier) (type_hyps : list (nat * (string * nat))) : option (Stack * Unifier) :=
+  match Σ, type_hyps with
+  | [], [] => Some ([], [])
+  | [], _  => None
+  | (Cst ty::τ)::Σ, (_, (ty', v))::type_hyps =>
+    if binds unifier v then None
+    else if (ty =? ty')%string then
+      unify Σ ((v, τ)::unifier) type_hyps
+    else None
+  | _, _ => None
+  end.
+
+Definition as_subst (unifier : Unifier) : (nat -> Term) :=
+  fun x =>
+    match get unifier x with
+    | None => [Var x]
+    | Some τ => τ
+    end.
+
+Notation "τ '.⟨' σ '⟩'" := (substitute τ (as_subst σ)) (at level 80).
+
+Fixpoint apply_unifier (unifier : Unifier) (Σ : Stack) : Stack :=
+  match Σ with
+  | [] => []
+  | τ::Σ =>
+    (substitute τ (as_subst unifier))::apply_unifier unifier Σ
+  end.
+
+Fixpoint term_eqb (τ1 τ2 : Term) : bool :=
+  match τ1, τ2 with
+  | [], [] => true
+  | (Cst x)::xs, (Cst y)::ys =>
+    (x =? y)%string && term_eqb xs ys
+  | (Var x)::xs, (Var y)::ys =>
+    (x =? y)%nat && term_eqb xs ys
+  | _, _ => false
+  end.
+
+Declare Scope term.
+Delimit Scope term with term.
+Notation "x =? y" := (term_eqb x y)%term.
+
+Fixpoint match_facts (Σ : Stack) (fact_hyps : list (nat * Term)) : option Stack :=
+  match Σ, fact_hyps with
+  | [], [] => Some []
+  | τ::Σ, (_, τ')::fact_hyps =>
+    if (τ =? τ')%term then
+      match_facts Σ fact_hyps
+    else
+      None
+  | _, _ => None
+  end.
+
+Inductive status :=
+  | UnificationFailed
+  | MatchingFailed
+  | StackUnderflow
+  | StackOverflow
+  | UndefinedType (id : nat)
+  | UndefinedFact (id : nat)
+  | UndefinedRule (id : nat)
+  | WrongStmt (τ : Term)
+  | Assumed (τ : Term)
+  | Proved (τ : Term).
+
+Definition term (s : Statement) : Term :=
+  match s with
+  | Ax τ => τ
+  | Th τ _ => τ
+  end.
+
+Fixpoint exec_proof (F : File) (Σ : Stack) type_hyps fact_hyps proof :=
+  match proof with
+  | [] =>
+    match Σ with
+    | [] => StackUnderflow
+    | [τ] => Proved τ
+    | _ => StackOverflow
+    end
+  | TypeLbl lbl::proof =>
+    match get type_hyps lbl with
+    | Some (ty, v) => exec_proof F ([Cst ty; Var v]::Σ) type_hyps fact_hyps proof
+    | None => UndefinedType lbl
+    end
+  | FactLbl lbl::proof =>
+    match get fact_hyps lbl with
+    | Some f => exec_proof F (f::Σ) type_hyps fact_hyps proof
+    | None => UndefinedFact lbl
+    end
+  | RuleLbl lbl::proof =>
+    match get (rules F) lbl with
+    | Some (RULE r_type_hyps r_fact_hyps r_stmt) =>
+      match unify Σ [] r_type_hyps with
+      | Some (Σ, unifier) =>
+        match match_facts (apply_unifier unifier Σ) r_fact_hyps with
+        | Some Σ => exec_proof F ((term r_stmt).⟨unifier⟩::Σ) type_hyps fact_hyps proof
+        | None => MatchingFailed
+        end
+      | None => UnificationFailed
+      end
+    | None => UndefinedRule lbl
+    end
+  end.
+
+Definition check (F : File) (R : Rule) : status :=
+  match statement R with
+  | Ax stmt => Assumed stmt
+  | Th stmt proof =>
+    match exec_proof F [] (type_hypothesis R) (fact_hypothesis R) proof with
+    | Proved stmt' =>
+      if (stmt =? stmt')%term then Proved stmt
+      else WrongStmt stmt'
+    | status => status
+    end
+  end.
+
+Example my_rule := RULE [(0, ("wff"%string, 0))] [] (Ax [Cst "a"; Var 0]).
+Example my_file := FILE [(0, my_rule)].
+Example my_thm := RULE [(0, ("wff"%string, 0))] [] (Th [Cst "a"; Var 0] [TypeLbl 0; RuleLbl 0]).
+Compute (check my_file my_thm).
+
+End Mm.
+
+
+Section Soundness.
+(* Definition interp_Rule (R : Rule) : Proposition := *)
+End Soundness.
